bedrock2/src/bedrock2/ProgramLogic.v
@@ -16,13 +16,17 @@ Lemma align_trace_cons {T} x xs cont t (H : xs = app cont t) : @cons T x xs = ap
 Proof. intros. cbn. congruence. Qed.
 Lemma align_trace_app {T} x xs cont t (H : xs = app cont t) : @app T x xs = app (app x cont) t.
 Proof. intros. cbn. subst. rewrite List.app_assoc; trivial. Qed.
+Check filterio. Print filterio.
+Lemma filterio_cons {width: BinNums.Z}{BW: Bitwidth.Bitwidth width}{word: Interface.word.word width}{mem: Interface.map.map Interface.word.rep Init.Byte.byte} (t : trace) (e : event) :
+  filterio (cons e t) = match e with | IO i => cons i (filterio t) | _ => filterio t end.
+Proof. destruct e; reflexivity. Qed.
 
 Ltac trace_alignment :=
     repeat match goal with
       | t := cons _ _ |- _ => subst t
       end;
     repeat match goal with
-      | H1 : filterio _ = _ |- context [ filterio _ ]  => (*idtac "12t";*) cbn [filterio List.flat_map]; rewrite H1
+      | H1 : filterio _ = _ |- context [ filterio _ ]  => repeat rewrite filterio_cons; repeat rewrite filterio_cons in H1; rewrite H1
       end;          
     repeat (eapply align_trace_app
       || eapply align_trace_cons
@@ -265,6 +269,8 @@ Ltac fwd_uniq_step :=
   end.
 Ltac fwd_uniq := repeat fwd_uniq_step.
 
+Check WeakestPrecondition.call. Check WeakestPrecondition.cmd.
+
 Ltac straightline :=
   match goal with
   | _ => idtac "1"; straightline_cleanup
@@ -275,42 +281,31 @@ Ltac straightline :=
       replace test with true by reflexivity; change T end;
                         cbv match beta delta [WeakestPrecondition.func]*)
   | |- program_logic_goal_for ?f _ =>
-        enter f; intros;
-         repeat
-          match goal with
-          | stack_addr:trace -> BinNums.Z -> ?word, H:?P ?functions |- _ =>
-                match type of functions with
-                | list (String.string * Syntax.func) =>
-                    let f := fresh "f" in
-                    pose proof (H stack_addr) as H; destruct H as [f H]
-                end
-          end;
-        match goal with
-        | |- call _ _ _ _ _ _ _ => idtac
-        | _ => eexists
-        end; intros; unfold1_call_goal; cbv beta match delta [call_body];
-        lazymatch goal with
-        | |- if ?test then ?T else _ => replace test with true by reflexivity; change T
-        end; cbv beta match delta [func]
-      (*idtac "2A";
       enter f; intros;
+      repeat
+        match goal with
+        | H:?P ?functions |- _ =>
+            match type of functions with
+            | list (String.string * Syntax.func) =>
+                let f := fresh "f" in destruct H as [f H]
+            end
+        end;
       match goal with
-      | |- call _ _ _ _ _ _ _ => idtac
-      | _ => eexists(*for ct case*)
+      | |- call _ _ _ _ _ _ => idtac
+      | _ => eexists
+      end; intros; unfold1_call_goal; cbv beta match delta [call_body];
+      lazymatch goal with
+      | |- if ?test then ?T else _ => replace test with true by reflexivity; change T
       end;
-      intros;
-      unfold1_call_goal; cbv match beta delta [call_body];
-                                   lazymatch goal with |- if ?test then ?T else _ =>
-                                                         replace test with true by reflexivity; change T end;
-                                                       cbv match beta delta [WeakestPrecondition.func]*)
-  | |- WeakestPrecondition.cmd _ _ (cmd.set ?s ?e) _ _ _ ?post => idtac "3";
+      cbv beta match delta [func]
+  | |- WeakestPrecondition.cmd _ (cmd.set ?s ?e) _ _ _ ?post => idtac "3";
     unfold1_cmd_goal; cbv beta match delta [cmd_body];
     let __ := match s with String.String _ _ => idtac | String.EmptyString => idtac end in
     ident_of_constr_string_cps s ltac:(fun x =>
       ensure_free x;
       (* NOTE: keep this consistent with the [exists _, _ /\ _] case far below *)
       letexists _ as x; split; [solve [repeat straightline]|])
-  | |- cmd _ _ ?c _ _ _ ?post => idtac "4";
+  | |- cmd _ ?c _ _ _ ?post => idtac "4";
     let c := eval hnf in c in
     lazymatch c with
     | cmd.while _ _ => fail
@@ -420,12 +415,14 @@ Ltac straightline :=
   | |- _ => idtac "43"; straightline_stackdealloc
   | |- context[sep (sep _ _) _] => idtac "44"; progress (flatten_seps_in_goal; cbn [seps])
   | H : context[sep (sep _ _) _] |- _ => idtac "45"; progress (flatten_seps_in H; cbn [seps] in H)
-  end.
+end.
 
+                                                       
+Check WeakestPrecondition.call.
 (* TODO: once we can automatically prove some calls, include the success-only version of this in [straightline] *)
 Ltac straightline_call :=
   lazymatch goal with
-  | |- WeakestPrecondition.call _ ?functions ?callee _ _ _ _ =>
+  | |- WeakestPrecondition.call ?functions ?callee _ _ _ _ =>
     let callee_spec := lazymatch constr:(_:spec_of callee) with ?s => s end in
     let Hcall := lazymatch goal with H: callee_spec functions |- _ => H end in
     eapply WeakestPreconditionProperties.Proper_call; cycle -1;
@@ -435,18 +432,18 @@ Ltac straightline_call :=
 
 Ltac straightline_ct_call :=
   lazymatch goal with
-  | |- call _ ?functions ?callee _ _ _ _ =>
+  | |- call ?functions ?callee _ _ _ _ =>
       let Hcall := multimatch goal with
-                   | H: context [ call _ functions callee _ _ _ _ ] |- _ => H
+                   | H: context [ call functions callee _ _ _ _ ] |- _ => H
                    end in
       eapply WeakestPreconditionProperties.Proper_call; cycle -1;
         [ eapply Hcall | try eabstract solve [ Morphisms.solve_proper ].. ];
         [ .. | intros ? ? ? ? ]
-  end.
+  end. Check WeakestPrecondition.cmd.
 
 Ltac current_trace_mem_locals :=
   lazymatch goal with
-  | |- WeakestPrecondition.cmd _ _ _ ?t ?m ?l _ => constr:((t, m, l))
+  | |- WeakestPrecondition.cmd _ _ ?t ?m ?l _ => constr:((t, m, l))
   end.
 
 Ltac seprewrite Hrw :=
