bedrock2/src/bedrock2Examples/FlatConstMem.v
@@ -28,7 +28,7 @@ Require Import coqutil.Tactics.rewr.
 Require Import AdmitAxiom.
 
 Section WithParameters.
-  Context {word: word.word 32} {mem: map.map word Byte.byte}.
+  Context {word: word.word 32} {mem: map.map word Byte.byte} {pick_sp: PickSp}.
   Context {word_ok: word.ok word} {mem_ok: map.ok mem}.
   Add Ring wring : (Properties.word.ring_theory (word := word))
         (preprocess [autorewrite with rew_word_morphism],
