bedrock2/src/bedrock2Examples/full_adder.v
@@ -17,6 +17,8 @@ From bedrock2 Require Import WeakestPrecondition ProgramLogic BasicC64Semantics.
 Import coqutil.Word.Interface.
 Require Import bedrock2.ZnWords.
 
+Context {pick_sp: Semantics.PickSp}. (* is there a better place to put this?*)
+
 Local Instance spec_of_add_with_carry : spec_of "add_with_carry" :=
   fnspec! "add_with_carry" x y carry ~> sum carry_out,
     { (* The required upper bound on `carry` isn't necessary for the
@@ -55,7 +57,7 @@ Proof.
   repeat
     (match goal with
      | X := _ |- _  => subst X end).
-  destruct (word.ltu (word.add x'0 carry) carry);
-    destruct (word.ltu (word.add (word.add x'0 carry) y) y);
+  destruct (word.ltu (word.add x carry) carry);
+    destruct (word.ltu (word.add (word.add x carry) y) y);
     ZnWords.
 Qed.
