bedrock2/src/bedrock2Examples/uint128_32.v
@@ -46,7 +46,7 @@ Require Import coqutil.Tactics.Tactics.
 Local Ltac invert H := inversion H; clear H.
 
 Section WithParameters.
-  Context {word: word.word 32} {mem: map.map word Byte.byte}.
+  Context {word: word.word 32} {mem: map.map word Byte.byte} {pick_sp: PickSp}.
   Context {word_ok: word.ok word} {mem_ok: map.ok mem}.
   Import ProgramLogic.Coercions.
   Local Number Notation nat Nat.of_num_uint Nat.to_num_hex_uint (abstract after 5001) : core_scope.
